Example.v
@@ -1,5 +1,7 @@
-Require Import Int31 List BasicRubik Rubik31 Solver.
-From Bignums Require Import BigN.
+(*
+Require Import Int31 List BasicRubik Rubik31 Solver31.
+*)
+Require Import Int63 List BasicRubik Rubik63 Solver63.
 
 (* Just to compute the state *)
 Time Eval native_compute in solve init_state.
